Port cav to ccelf, pass the test
1. fix bug in addrmode (E4 and E6)
2. add lots of unsupported instruction
3. lots of wrong operand order in "_rr" instruction, fix them
4. bug found in encode_ofs_u16

autogen/EncDecRet.v
@@ -1,6 +1,6 @@
 Require Import Coqlib Integers Errors.
 Require Import encode.Hex encode.Bits Memdata.
-Require Import Encode VerificationCondition.
+Require Import Encode  VerificationCondition.
 Import String Ascii.
 Import List.
 Import ListNotations.
@@ -278,7 +278,7 @@ Hint Unfold read_B write_B read_R write_R read_W write_W read_X write_X read_bas
 
 Hint Unfold AddrE12_bp AddrE11_bp AddrE10_bp AddrE9_bp AddrE8_bp AddrE7_bp AddrE6_bp AddrE5_bp AddrE4_bp AddrE0_bp :AddrE_bpdb.
 
-Hint Unfold Ptestq_EvGv_bp Ptestq_ri_bp Pcmpq_GvEv_bp Pcmpq_EvGv_bp Pcmpq_ri_bp Prorq_ri_bp Psarq_ri_bp Psarq_rcl_bp Psalq_ri_bp Psalq_rcl_bp Pnotq_bp Pxorq_GvEv_bp Pxorq_EvGv_bp Pxorq_ri_bp Porq_GvEv_bp Porq_EvGv_bp Porq_ri_bp Pandq_GvEv_bp Pandq_EvGv_bp Pandq_ri_bp Pdivq_bp Pidivq_bp Pmulq_r_bp Pimulq_GvEv_bp Pimulq_r_bp Pimulq_ri_bp Psubq_GvEv_bp Psubq_EvGv_bp Psubq_ri_bp Paddq_GvEv_bp Paddq_EvGv_bp Paddq_ri_bp Pnegq_bp Pleaq_bp Pmovq_EvGv_bp Pmovq_GvEv_bp Pmovq_ri_bp Psubl_ri_bp Pbsqrtsd_bp Psbbl_rr_bp Prep_movsl_bp Pmovsq_rm_bp Pmovsq_mr_bp Pminsd_bp Pmaxsd_bp Pbswap32_bp Pbsrl_bp Pbsfl_bp Paddl_mi_bp Paddl_rr_bp Padcl_rr_bp Padcl_ri_bp Pjcc_rel_bp Pret_iw_bp Pret_bp Pcall_r_bp Pcall_ofs_bp Pnop_bp Pjmp_Ev_bp Pjmp_l_rel_bp Pandps_fm_bp Pxorps_GvEv_bp Pxorpd_GvEv_bp Pcomiss_ff_bp Pcomisd_ff_bp Pdivss_ff_bp Pdivsd_ff_bp Pmuls_ff_bp Pmuld_ff_bp Psubs_ff_bp Psubd_ff_bp Padds_ff_bp Paddd_ff_bp Psetcc_bp Pcmov_bp Ptestl_rr_bp Ptestl_ri_bp Pcmpl_ri_bp Pcmpl_rr_bp Prorl_ri_bp Prolw_ri_bp Pshld_ri_bp Psarl_rcl_bp Psarl_ri_bp Pshrl_rcl_bp Pshrl_ri_bp Psall_rcl_bp Psall_ri_bp Pnotl_bp Pxorl_rr_bp Pxorl_ri_bp Porl_rr_bp Porl_ri_bp Pandl_ri_bp Pandl_rr_bp Pidivl_r_bp Pdivl_r_bp Pcltd_bp Pmull_r_bp Pimull_r_bp Pimull_ri_bp Pimull_rr_bp Psubl_rr_bp Paddl_ri_bp Pnegl_bp Pleal_bp Pcvttss2si_rf_bp Pcvtsi2sd_fr_bp Pcvtsi2ss_fr_bp Pcvttsd2si_rf_bp Pcvtss2sd_ff_bp Pcvtsd2ss_ff_bp Pmovsw_GvEv_bp Pmovzw_GvEv_bp Pmovsb_GvEv_bp Pmovzb_rm_bp Pmovw_rm_bp Pmovw_mr_bp Pmovb_rm_bp Pmovb_mr_bp Pxchg_rr_bp Pflds_m_bp Pfstps_m_bp Pfstpl_m_bp Pfldl_m_bp Pmovss_fm_bp Pmovss_mf_bp Pmovsd_fm_bp Pmovsd_mf_bp Pmovl_rm_bp Pmovl_mr_bp Pmovl_ri_bp :Instruction_bpdb.
+Hint Unfold Ptestq_EvGv_bp Ptestq_ri_bp Pcmpq_GvEv_bp Pcmpq_EvGv_bp Pcmpq_ri_bp Prorq_ri_bp Psarq_ri_bp Psarq_rcl_bp Psalq_ri_bp Psalq_rcl_bp Pnotq_bp Pxorq_GvEv_bp Pxorq_EvGv_bp Pxorq_ri_bp Porq_GvEv_bp Porq_EvGv_bp Porq_ri_bp Pandq_GvEv_bp Pandq_EvGv_bp Pandq_ri_bp Pdivq_bp Pidivq_bp Pmulq_r_bp Pimulq_GvEv_bp Pimulq_r_bp Pimulq_ri_bp Psubq_GvEv_bp Psubq_EvGv_bp Psubq_ri_bp Paddq_GvEv_bp Paddq_EvGv_bp Paddq_ri_bp Pnegq_bp Pleaq_bp Pmovq_EvGv_bp Pmovq_GvEv_bp Pmovq_ri_bp Psubl_ri_bp Pbsqrtsd_bp Psbbl_rr_bp Prep_movsl_bp Pmovsq_rm_bp Pmovsq_mr_bp Pminsd_bp Pmaxsd_bp Pbswap32_bp Pbsrl_bp Pbsfl_bp Paddl_mi_bp Paddl_rr_bp Padcl_rr_bp Padcl_ri_bp Pjcc_rel_bp Pret_iw_bp Pret_bp Pcall_r_bp Pcall_ofs_bp Pnop_bp Pjmp_Ev_bp Pjmp_l_rel_bp Pandps_fm_bp Pxorps_GvEv_bp Pxorpd_GvEv_bp Pcomiss_ff_bp Pcomisd_ff_bp Pdivss_ff_bp Pdivsd_ff_bp Pmuls_ff_bp Pmuld_ff_bp Psubs_ff_bp Psubd_ff_bp Pandpd_GvEv_bp Padds_ff_bp Paddd_ff_bp Psetcc_bp Pcmov_bp Ptestl_rr_bp Ptestl_ri_bp Pcmpl_ri_bp Pcmpl_rr_bp Prorl_ri_bp Prolw_ri_bp Pshld_ri_bp Psarl_rcl_bp Psarl_ri_bp Pshrl_rcl_bp Pshrl_ri_bp Psall_rcl_bp Psall_ri_bp Pnotl_bp Pxorl_rr_bp Pxorl_ri_bp Porl_rr_bp Porl_ri_bp Pandl_ri_bp Pandl_rr_bp Pidivl_r_bp Pdivl_r_bp Pcltd_bp Pmull_r_bp Pimull_r_bp Pimull_ri_bp Pimull_rr_bp Psubl_rr_bp Paddl_ri_bp Pnegl_bp Pleal_bp Pcvttss2si_rf_bp Pcvtsi2sd_fr_bp Pcvtsi2ss_fr_bp Pcvttsd2si_rf_bp Pcvtss2sd_ff_bp Pcvtsd2ss_ff_bp Pmovsw_GvEv_bp Pmovzw_GvEv_bp Pmovsb_GvEv_bp Pmovzb_rm_bp Pmovw_rm_bp Pmovw_mr_bp Pmovb_rm_bp Pmovb_mr_bp Pxchg_rr_bp Pflds_m_bp Pfstps_m_bp Pfstpl_m_bp Pfldl_m_bp Pmovss_fm_bp Pmovss_mf_bp Pmovsd_fm_bp Pmovsd_mf_bp Pmovl_rm_bp Pmovl_mr_bp Pmovl_ri_bp :Instruction_bpdb.
 Lemma AddrE_bp_in_list0: 
 In AddrE12_bp AddrE_bp_list.
 Proof.
@@ -685,306 +685,311 @@ Proof.
 simpl; goOver; auto. Qed.
 
 Lemma Instruction_bp_in_list71: 
-In Padds_ff_bp Instruction_bp_list.
+In Pandpd_GvEv_bp Instruction_bp_list.
 Proof.
 simpl; goOver; auto. Qed.
 
 Lemma Instruction_bp_in_list72: 
-In Paddd_ff_bp Instruction_bp_list.
+In Padds_ff_bp Instruction_bp_list.
 Proof.
 simpl; goOver; auto. Qed.
 
 Lemma Instruction_bp_in_list73: 
-In Psetcc_bp Instruction_bp_list.
+In Paddd_ff_bp Instruction_bp_list.
 Proof.
 simpl; goOver; auto. Qed.
 
 Lemma Instruction_bp_in_list74: 
-In Pcmov_bp Instruction_bp_list.
+In Psetcc_bp Instruction_bp_list.
 Proof.
 simpl; goOver; auto. Qed.
 
 Lemma Instruction_bp_in_list75: 
-In Ptestl_rr_bp Instruction_bp_list.
+In Pcmov_bp Instruction_bp_list.
 Proof.
 simpl; goOver; auto. Qed.
 
 Lemma Instruction_bp_in_list76: 
-In Ptestl_ri_bp Instruction_bp_list.
+In Ptestl_rr_bp Instruction_bp_list.
 Proof.
 simpl; goOver; auto. Qed.
 
 Lemma Instruction_bp_in_list77: 
-In Pcmpl_ri_bp Instruction_bp_list.
+In Ptestl_ri_bp Instruction_bp_list.
 Proof.
 simpl; goOver; auto. Qed.
 
 Lemma Instruction_bp_in_list78: 
-In Pcmpl_rr_bp Instruction_bp_list.
+In Pcmpl_ri_bp Instruction_bp_list.
 Proof.
 simpl; goOver; auto. Qed.
 
 Lemma Instruction_bp_in_list79: 
-In Prorl_ri_bp Instruction_bp_list.
+In Pcmpl_rr_bp Instruction_bp_list.
 Proof.
 simpl; goOver; auto. Qed.
 
 Lemma Instruction_bp_in_list80: 
-In Prolw_ri_bp Instruction_bp_list.
+In Prorl_ri_bp Instruction_bp_list.
 Proof.
 simpl; goOver; auto. Qed.
 
 Lemma Instruction_bp_in_list81: 
-In Pshld_ri_bp Instruction_bp_list.
+In Prolw_ri_bp Instruction_bp_list.
 Proof.
 simpl; goOver; auto. Qed.
 
 Lemma Instruction_bp_in_list82: 
-In Psarl_rcl_bp Instruction_bp_list.
+In Pshld_ri_bp Instruction_bp_list.
 Proof.
 simpl; goOver; auto. Qed.
 
 Lemma Instruction_bp_in_list83: 
-In Psarl_ri_bp Instruction_bp_list.
+In Psarl_rcl_bp Instruction_bp_list.
 Proof.
 simpl; goOver; auto. Qed.
 
 Lemma Instruction_bp_in_list84: 
-In Pshrl_rcl_bp Instruction_bp_list.
+In Psarl_ri_bp Instruction_bp_list.
 Proof.
 simpl; goOver; auto. Qed.
 
 Lemma Instruction_bp_in_list85: 
-In Pshrl_ri_bp Instruction_bp_list.
+In Pshrl_rcl_bp Instruction_bp_list.
 Proof.
 simpl; goOver; auto. Qed.
 
 Lemma Instruction_bp_in_list86: 
-In Psall_rcl_bp Instruction_bp_list.
+In Pshrl_ri_bp Instruction_bp_list.
 Proof.
 simpl; goOver; auto. Qed.
 
 Lemma Instruction_bp_in_list87: 
-In Psall_ri_bp Instruction_bp_list.
+In Psall_rcl_bp Instruction_bp_list.
 Proof.
 simpl; goOver; auto. Qed.
 
 Lemma Instruction_bp_in_list88: 
-In Pnotl_bp Instruction_bp_list.
+In Psall_ri_bp Instruction_bp_list.
 Proof.
 simpl; goOver; auto. Qed.
 
 Lemma Instruction_bp_in_list89: 
-In Pxorl_rr_bp Instruction_bp_list.
+In Pnotl_bp Instruction_bp_list.
 Proof.
 simpl; goOver; auto. Qed.
 
 Lemma Instruction_bp_in_list90: 
-In Pxorl_ri_bp Instruction_bp_list.
+In Pxorl_rr_bp Instruction_bp_list.
 Proof.
 simpl; goOver; auto. Qed.
 
 Lemma Instruction_bp_in_list91: 
-In Porl_rr_bp Instruction_bp_list.
+In Pxorl_ri_bp Instruction_bp_list.
 Proof.
 simpl; goOver; auto. Qed.
 
 Lemma Instruction_bp_in_list92: 
-In Porl_ri_bp Instruction_bp_list.
+In Porl_rr_bp Instruction_bp_list.
 Proof.
 simpl; goOver; auto. Qed.
 
 Lemma Instruction_bp_in_list93: 
-In Pandl_ri_bp Instruction_bp_list.
+In Porl_ri_bp Instruction_bp_list.
 Proof.
 simpl; goOver; auto. Qed.
 
 Lemma Instruction_bp_in_list94: 
-In Pandl_rr_bp Instruction_bp_list.
+In Pandl_ri_bp Instruction_bp_list.
 Proof.
 simpl; goOver; auto. Qed.
 
 Lemma Instruction_bp_in_list95: 
-In Pidivl_r_bp Instruction_bp_list.
+In Pandl_rr_bp Instruction_bp_list.
 Proof.
 simpl; goOver; auto. Qed.
 
 Lemma Instruction_bp_in_list96: 
-In Pdivl_r_bp Instruction_bp_list.
+In Pidivl_r_bp Instruction_bp_list.
 Proof.
 simpl; goOver; auto. Qed.
 
 Lemma Instruction_bp_in_list97: 
-In Pcltd_bp Instruction_bp_list.
+In Pdivl_r_bp Instruction_bp_list.
 Proof.
 simpl; goOver; auto. Qed.
 
 Lemma Instruction_bp_in_list98: 
-In Pmull_r_bp Instruction_bp_list.
+In Pcltd_bp Instruction_bp_list.
 Proof.
 simpl; goOver; auto. Qed.
 
 Lemma Instruction_bp_in_list99: 
-In Pimull_r_bp Instruction_bp_list.
+In Pmull_r_bp Instruction_bp_list.
 Proof.
 simpl; goOver; auto. Qed.
 
 Lemma Instruction_bp_in_list100: 
-In Pimull_ri_bp Instruction_bp_list.
+In Pimull_r_bp Instruction_bp_list.
 Proof.
 simpl; goOver; auto. Qed.
 
 Lemma Instruction_bp_in_list101: 
-In Pimull_rr_bp Instruction_bp_list.
+In Pimull_ri_bp Instruction_bp_list.
 Proof.
 simpl; goOver; auto. Qed.
 
 Lemma Instruction_bp_in_list102: 
-In Psubl_rr_bp Instruction_bp_list.
+In Pimull_rr_bp Instruction_bp_list.
 Proof.
 simpl; goOver; auto. Qed.
 
 Lemma Instruction_bp_in_list103: 
-In Paddl_ri_bp Instruction_bp_list.
+In Psubl_rr_bp Instruction_bp_list.
 Proof.
 simpl; goOver; auto. Qed.
 
 Lemma Instruction_bp_in_list104: 
-In Pnegl_bp Instruction_bp_list.
+In Paddl_ri_bp Instruction_bp_list.
 Proof.
 simpl; goOver; auto. Qed.
 
 Lemma Instruction_bp_in_list105: 
-In Pleal_bp Instruction_bp_list.
+In Pnegl_bp Instruction_bp_list.
 Proof.
 simpl; goOver; auto. Qed.
 
 Lemma Instruction_bp_in_list106: 
-In Pcvttss2si_rf_bp Instruction_bp_list.
+In Pleal_bp Instruction_bp_list.
 Proof.
 simpl; goOver; auto. Qed.
 
 Lemma Instruction_bp_in_list107: 
-In Pcvtsi2sd_fr_bp Instruction_bp_list.
+In Pcvttss2si_rf_bp Instruction_bp_list.
 Proof.
 simpl; goOver; auto. Qed.
 
 Lemma Instruction_bp_in_list108: 
-In Pcvtsi2ss_fr_bp Instruction_bp_list.
+In Pcvtsi2sd_fr_bp Instruction_bp_list.
 Proof.
 simpl; goOver; auto. Qed.
 
 Lemma Instruction_bp_in_list109: 
-In Pcvttsd2si_rf_bp Instruction_bp_list.
+In Pcvtsi2ss_fr_bp Instruction_bp_list.
 Proof.
 simpl; goOver; auto. Qed.
 
 Lemma Instruction_bp_in_list110: 
-In Pcvtss2sd_ff_bp Instruction_bp_list.
+In Pcvttsd2si_rf_bp Instruction_bp_list.
 Proof.
 simpl; goOver; auto. Qed.
 
 Lemma Instruction_bp_in_list111: 
-In Pcvtsd2ss_ff_bp Instruction_bp_list.
+In Pcvtss2sd_ff_bp Instruction_bp_list.
 Proof.
 simpl; goOver; auto. Qed.
 
 Lemma Instruction_bp_in_list112: 
-In Pmovsw_GvEv_bp Instruction_bp_list.
+In Pcvtsd2ss_ff_bp Instruction_bp_list.
 Proof.
 simpl; goOver; auto. Qed.
 
 Lemma Instruction_bp_in_list113: 
-In Pmovzw_GvEv_bp Instruction_bp_list.
+In Pmovsw_GvEv_bp Instruction_bp_list.
 Proof.
 simpl; goOver; auto. Qed.
 
 Lemma Instruction_bp_in_list114: 
-In Pmovsb_GvEv_bp Instruction_bp_list.
+In Pmovzw_GvEv_bp Instruction_bp_list.
 Proof.
 simpl; goOver; auto. Qed.
 
 Lemma Instruction_bp_in_list115: 
-In Pmovzb_rm_bp Instruction_bp_list.
+In Pmovsb_GvEv_bp Instruction_bp_list.
 Proof.
 simpl; goOver; auto. Qed.
 
 Lemma Instruction_bp_in_list116: 
-In Pmovw_rm_bp Instruction_bp_list.
+In Pmovzb_rm_bp Instruction_bp_list.
 Proof.
 simpl; goOver; auto. Qed.
 
 Lemma Instruction_bp_in_list117: 
-In Pmovw_mr_bp Instruction_bp_list.
+In Pmovw_rm_bp Instruction_bp_list.
 Proof.
 simpl; goOver; auto. Qed.
 
 Lemma Instruction_bp_in_list118: 
-In Pmovb_rm_bp Instruction_bp_list.
+In Pmovw_mr_bp Instruction_bp_list.
 Proof.
 simpl; goOver; auto. Qed.
 
 Lemma Instruction_bp_in_list119: 
-In Pmovb_mr_bp Instruction_bp_list.
+In Pmovb_rm_bp Instruction_bp_list.
 Proof.
 simpl; goOver; auto. Qed.
 
 Lemma Instruction_bp_in_list120: 
-In Pxchg_rr_bp Instruction_bp_list.
+In Pmovb_mr_bp Instruction_bp_list.
 Proof.
 simpl; goOver; auto. Qed.
 
 Lemma Instruction_bp_in_list121: 
-In Pflds_m_bp Instruction_bp_list.
+In Pxchg_rr_bp Instruction_bp_list.
 Proof.
 simpl; goOver; auto. Qed.
 
 Lemma Instruction_bp_in_list122: 
-In Pfstps_m_bp Instruction_bp_list.
+In Pflds_m_bp Instruction_bp_list.
 Proof.
 simpl; goOver; auto. Qed.
 
 Lemma Instruction_bp_in_list123: 
-In Pfstpl_m_bp Instruction_bp_list.
+In Pfstps_m_bp Instruction_bp_list.
 Proof.
 simpl; goOver; auto. Qed.
 
 Lemma Instruction_bp_in_list124: 
-In Pfldl_m_bp Instruction_bp_list.
+In Pfstpl_m_bp Instruction_bp_list.
 Proof.
 simpl; goOver; auto. Qed.
 
 Lemma Instruction_bp_in_list125: 
-In Pmovss_fm_bp Instruction_bp_list.
+In Pfldl_m_bp Instruction_bp_list.
 Proof.
 simpl; goOver; auto. Qed.
 
 Lemma Instruction_bp_in_list126: 
-In Pmovss_mf_bp Instruction_bp_list.
+In Pmovss_fm_bp Instruction_bp_list.
 Proof.
 simpl; goOver; auto. Qed.
 
 Lemma Instruction_bp_in_list127: 
-In Pmovsd_fm_bp Instruction_bp_list.
+In Pmovss_mf_bp Instruction_bp_list.
 Proof.
 simpl; goOver; auto. Qed.
 
 Lemma Instruction_bp_in_list128: 
-In Pmovsd_mf_bp Instruction_bp_list.
+In Pmovsd_fm_bp Instruction_bp_list.
 Proof.
 simpl; goOver; auto. Qed.
 
 Lemma Instruction_bp_in_list129: 
-In Pmovl_rm_bp Instruction_bp_list.
+In Pmovsd_mf_bp Instruction_bp_list.
 Proof.
 simpl; goOver; auto. Qed.
 
 Lemma Instruction_bp_in_list130: 
-In Pmovl_mr_bp Instruction_bp_list.
+In Pmovl_rm_bp Instruction_bp_list.
 Proof.
 simpl; goOver; auto. Qed.
 
 Lemma Instruction_bp_in_list131: 
+In Pmovl_mr_bp Instruction_bp_list.
+Proof.
+simpl; goOver; auto. Qed.
+
+Lemma Instruction_bp_in_list132: 
 In Pmovl_ri_bp Instruction_bp_list.
 Proof.
 simpl; goOver; auto. Qed.
@@ -1384,6 +1389,7 @@ Inductive Instruction: Type :=
 | Pmuld_ff(uvar3_0:u3)(uvar3_1:u3)
 | Psubs_ff(uvar3_0:u3)(uvar3_1:u3)
 | Psubd_ff(uvar3_0:u3)(uvar3_1:u3)
+| Pandpd_GvEv(AddrE:AddrE)(uvar3_0:u3)
 | Padds_ff(uvar3_0:u3)(uvar3_1:u3)
 | Paddd_ff(uvar3_0:u3)(uvar3_1:u3)
 | Psetcc(uvar4_0:u4)(uvar3_1:u3)
@@ -1517,6 +1523,7 @@ Inductive Instruction_op: Type :=
 | Pmuld_ff_op
 | Psubs_ff_op
 | Psubd_ff_op
+| Pandpd_GvEv_op
 | Padds_ff_op
 | Paddd_ff_op
 | Psetcc_op
@@ -1651,6 +1658,7 @@ Definition Instruction_to_op element  :=
 | Pmuld_ff _ _ => Pmuld_ff_op
 | Psubs_ff _ _ => Psubs_ff_op
 | Psubd_ff _ _ => Psubd_ff_op
+| Pandpd_GvEv _ _ => Pandpd_GvEv_op
 | Padds_ff _ _ => Padds_ff_op
 | Paddd_ff _ _ => Paddd_ff_op
 | Psetcc _ _ => Psetcc_op
@@ -1786,6 +1794,7 @@ Definition Instruction_op_to_bp element  :=
 | Pmuld_ff_op => Pmuld_ff_bp
 | Psubs_ff_op => Psubs_ff_bp
 | Psubd_ff_op => Psubd_ff_bp
+| Pandpd_GvEv_op => Pandpd_GvEv_bp
 | Padds_ff_op => Padds_ff_bp
 | Paddd_ff_op => Paddd_ff_bp
 | Psetcc_op => Psetcc_bp
@@ -2709,6 +2718,17 @@ let byte31 := write_mod byte30 b["11"] in
 let byte32 := write_reg_op byte31 (proj1_sig uvar3_0) in
 let byte33 := write_rm byte32 (proj1_sig uvar3_1) in
 let result3 := [byte33] in
+OK (result0 ++ result1 ++ result2 ++ result3)
+| Pandpd_GvEv AddrE uvar3_0 => let byte01 := HB["66"] in
+let result0 := [byte01] in
+let byte11 := HB["0F"] in
+let result1 := [byte11] in
+let byte21 := HB["58"] in
+let result2 := [byte21] in
+let byte30 := HB["00"] in
+let byte31 := write_reg_op byte30 (proj1_sig uvar3_0) in
+do byte32 <- encode_AddrE AddrE byte31;
+let result3 := byte32 in
 OK (result0 ++ result1 ++ result2 ++ result3)
 | Padds_ff uvar3_0 uvar3_1 => let byte01 := HB["F3"] in
 let result0 := [byte01] in
@@ -4552,6 +4572,20 @@ if assertLength uvar3_1 3 then
 do bytes4 <- try_skip_n bytes3 1;
 OK ((Psubd_ff (uvar3_0) (uvar3_1)), 4)
 else Error(msg"impossible")
+else Error(msg"impossible")
+else
+
+	if Pandpd_GvEv_bp bin then
+let bytes0 := code in
+do bytes1 <- try_skip_n bytes0 1;
+do bytes2 <- try_skip_n bytes1 1;
+do bytes3 <- try_skip_n bytes2 1;
+do byte0 <- try_get_n bytes3 0;
+let uvar3_0 := read_reg_op byte0 in
+if assertLength uvar3_0 3 then
+do (AddrE, localLength0) <- decode_AddrE bytes3;
+do bytes4 <- try_skip_n bytes3 localLength0;
+OK ((Pandpd_GvEv AddrE (uvar3_0)), 3 + localLength0)
 else Error(msg"impossible")
 else
 
